Lean4Lean/Verify/Environment.lean
@@ -1,5 +1,5 @@
 import Lean4Lean.Verify.LocalContext
-import Lean4Lean.Theory.Typing.Env
+import Lean4Lean.Theory.Typing.EnvLemmas
 
 namespace Lean4Lean
 open Lean
@@ -9,26 +9,99 @@ def isAsSafeAs : DefinitionSafety → ConstantInfo → Bool
   | .partial, ci => !ci.isUnsafe
   | .safe, ci => !ci.isUnsafe && !ci.isPartial
 
-variable (safety : DefinitionSafety) (ci : ConstantInfo) in
-inductive TrConstant : Option VConstant → Prop where
-  | safe : isAsSafeAs safety ci →
-    ci.levelParams.length = ci'.uvars →
-    TrExpr ci.levelParams [] ci.type ci'.type →
-    TrConstant (some ci')
-  | «unsafe» : ¬isAsSafeAs safety ci → TrConstant none
+def TrConstant (safety : DefinitionSafety) (ci : ConstantInfo) (ci' : VConstant) : Prop :=
+  isAsSafeAs safety ci ∧ ci.levelParams.length = ci'.uvars ∧
+  TrExpr ci.levelParams [] ci.type ci'.type
 
-def TrRecDefEq : RecursorVal → RecursorRule → VDefEq → Prop := sorry
+def TrConstVal (safety : DefinitionSafety) (ci : ConstantInfo) (ci' : VConstVal) : Prop :=
+  TrConstant safety ci ci'.toVConstant ∧ ci.name = ci'.name
 
-def TrDefEq : ConstantInfo → VDefEq → Prop
-  | .defnInfo ci, df => ∃ ty' val',
-    TrExpr ci.levelParams [] ci.type ty' ∧
-    TrExpr ci.levelParams [] ci.value val' ∧
-    df = VDefVal.toDefEq ⟨⟨⟨ci.levelParams.length, ty'⟩, ci.name⟩, val'⟩
-  | .quotInfo _, df => df = quotDefEq
-  | .recInfo ci, df => ∃ rule ∈ ci.rules, TrRecDefEq ci rule df
-  | _, _ => False
+def TrDefVal (safety : DefinitionSafety) (ci : ConstantInfo) (ci' : VDefVal) : Prop :=
+  TrConstVal safety ci ci'.toVConstVal ∧
+  TrExpr ci.levelParams [] ci.value! ci'.value
 
-structure TrEnv (safety : DefinitionSafety) (env : Environment) (venv : VEnv) : Prop where
-  constants : env.find? n = some ci →
-    ∃ ci', TrConstant safety ci ci' ∧ venv.constants n = some ci'
-  defeqs : venv.defeqs df ↔ ∃ ci, isAsSafeAs safety ci ∧ TrDefEq ci df
+def AddQuot1 (name : Name) (kind : QuotKind) (ci' : VConstant) (P : ConstMap → Prop)
+    (m : ConstMap) : Prop :=
+  ∃ levelParams type,
+    let ci := .quotInfo { name, kind, levelParams, type }
+    TrConstant .safe ci ci' ∧
+    P (m.insert name ci)
+
+def AddQuot (m1 m2 : ConstMap) : Prop :=
+  AddQuot1 ``Quot .type quotConst (m := m1) <|
+  AddQuot1 ``Quot.mk .ctor quotMkConst <|
+  AddQuot1 ``Quot.lift .lift quotLiftConst <|
+  AddQuot1 ``Quot.ind .ind quotMkConst (Eq m2)
+
+def AddInduct (m1 : ConstMap) (decl : VInductDecl) (m2 : ConstMap) : Prop := sorry
+
+variable (safety : DefinitionSafety) in
+inductive TrEnv' : ConstMap → Bool → VEnv → Prop where
+  | empty : TrEnv' {} false .empty
+  | block :
+    ¬isAsSafeAs safety ci →
+    env.addConst ci.name none = some env' →
+    TrEnv' C Q env →
+    TrEnv' (C.insert ci.name ci) Q env'
+  | axiom :
+    TrConstant safety (.axiomInfo ci) ci' →
+    ci'.WF env →
+    env.addConst ci.name (some ci') = some env' →
+    TrEnv' C Q env →
+    TrEnv' (C.insert ci.name (.axiomInfo ci)) Q env'
+  | defn {ci' : VDefVal} :
+    TrDefVal safety (.defnInfo ci) ci' →
+    ci'.WF env →
+    env.addConst ci.name (some ci'.toVConstant) = some env' →
+    TrEnv' C Q env →
+    TrEnv' (C.insert ci.name (.defnInfo ci)) Q (env'.addDefEq ci'.toDefEq)
+  | opaque {ci' : VDefVal} :
+    TrDefVal safety (.opaqueInfo ci) ci' →
+    ci'.WF env →
+    env.addConst ci.name (some ci'.toVConstant) = some env' →
+    TrEnv' C Q env →
+    TrEnv' (C.insert ci.name (.opaqueInfo ci)) Q env'
+  | quot :
+    env.QuotReady →
+    env.addQuot = some env' →
+    AddQuot C C' →
+    TrEnv' C false env →
+    TrEnv' C' true env'
+  | induct :
+    decl.WF env →
+    env.addInduct decl = some env' →
+    AddInduct C decl C' →
+    TrEnv' C Q env →
+    TrEnv' C' Q env'
+
+def TrEnv (safety : DefinitionSafety) (env : Environment) (venv : VEnv) : Prop :=
+  TrEnv' safety env.constants env.header.quotInit venv
+
+theorem TrEnv'.WF (H : TrEnv' C Q env venv) : ∃ ds, venv.WF ds := by
+  induction H with
+  | empty => exact ⟨_, .empty⟩
+  | block _ h _ ih =>
+    have ⟨_, H⟩ := ih
+    exact ⟨_, H.decl <| .block h⟩
+  | «axiom» _ h1 h2 _ ih =>
+    have ⟨_, H⟩ := ih
+    exact ⟨_, H.decl <| .axiom (ci := ⟨_, _⟩) h1 h2⟩
+  | defn h1 h2 h3 _ ih =>
+    have ⟨_, H⟩ := ih
+    have := h1.1.2; dsimp [ConstantInfo.name, ConstantInfo.toConstantVal] at this
+    exact ⟨_, H.decl <| .def h2 (this ▸ h3)⟩
+  | «opaque» h1 h2 h3 _ ih =>
+    have ⟨_, H⟩ := ih
+    have := h1.1.2; dsimp [ConstantInfo.name, ConstantInfo.toConstantVal] at this
+    exact ⟨_, H.decl <| .opaque h2 (this ▸ h3)⟩
+  | quot h1 h2 _ _ ih =>
+    have ⟨_, H⟩ := ih
+    exact ⟨_, H.decl <| .quot h1 h2⟩
+  | induct h1 h2 _ _ ih =>
+    have ⟨_, H⟩ := ih
+    exact ⟨_, H.decl <| .induct h1 h2⟩
+
+nonrec theorem TrEnv.WF (H : TrEnv safety env venv) : ∃ ds, venv.WF ds := H.WF
+
+theorem TrEnv.ordered (H : TrEnv safety env venv) : venv.Ordered :=
+  let ⟨_, H⟩ := H.WF; H.ordered
